FlowrefDecompiler.lean
@@ -215,7 +215,8 @@ def emitC (a : A) (bits : Bits) (insns : Array Ins) (fnVa : Nat) : IO (String ×
                                ∨ i.mn == "neg" ∨ i.mn == "not"
                                ∨ i.mn == "adc" ∨ i.mn == "sbb"
                                ∨ i.mn == "ror" ∨ i.mn == "rol" ∨ i.mn == "bswap"
-                               ∨ i.mn == "bsf" ∨ i.mn == "rep bsf" ∨ i.mn == "tzcnt" ∨ i.mn == "bsr" ∨ i.mn == "lzcnt")
+                               ∨ i.mn == "bsf" ∨ i.mn == "rep bsf" ∨ i.mn == "tzcnt" ∨ i.mn == "bsr" ∨ i.mn == "lzcnt"
+                               ∨ i.mn == "div" ∨ i.mn == "idiv")
                                ∧ ¬ (firstTok i).any (· == '[')
                           then some (firstTok i) else none
                 | _    => none
